# T5

* $$
  f'(x)=2(x-1)(x-3)^2+2(x-1)^2(x-3)\\=(x-1)(x-3)(2x-6+2x-2)\\=4(x-1)(x-2)(x-3)
  $$

* $$
  \Rightarrow f'(1)=f'(2)=f'(3),\\由罗尔定理得，\exist\xi_1\in(1,2),\exist\xi_2\in(2,3)使得f''(\xi_1)=0,f''(\xi_2)=0\\
  $$

* $$
  由于f(x)是四阶表达式，所以f''(x)为二阶表达式\\f''(x)有两个根\xi_1,\xi_2
  $$

* $$
  f''(x)=4(x-2)(x-3)+4(x-1)(x-3)+4(x-1)(x-2)\\=4(3x^2-12x+11)
  $$

* $$
  设f''(x)=12(x-\xi_1)(x-\xi_2),可知在\xi_1,\xi_2左右f''(x)变号
  $$

* $$
  拐点2
  $$

* 



# T4

* $$
  f(x)=ln[2(1+\frac{x}{2})]=ln2+ln(1+\frac{x}{2})\\=ln2+\frac{x}{2}-\frac{1}{2}(\frac{x}{2})^2+\frac{1}{3}(\frac{x}{2})^3+……
  $$

* $$
  ln(1+x)=\sum_{n=1}^{\infty}(-1)^{n-1}\frac{x^n}{n}=x-\frac{1}{2}x^2+\frac{1}{3}x^3-……+(-1)^{n-1}\frac{x^n}{n}+……，-1<x\leq1
  $$

* $$
  lnx^{(n)}=(-1)^{n-1}\frac{(n-1)!}{x^n},x=1,2,……
  $$

* $$
  f(x)=\sum_{n=0}^{\infty}\frac{f^{(n)}(0)}{n!}x^n\\或者f(x)=\sum_{n=0}^{\infty}\frac{f^{(n)}(x_0)}{n!}(x-x_0)^n
  $$

* $$
  \Rightarrow \frac{1}{3}(\frac{x}{2})^3=\frac{f'''(0)}{3!}x^3
  $$

* $$
  f'''(0)=\frac{1}{4}
  $$



# T3

* $$
  反证法：设\sum_{n=1}^{\infty}(|a_n|+|b_n|)收敛，\\由于0\leq|a_n|\leq|a_n|+|b_n|\Rightarrow\sum_{n=1}^{\infty}|a_n|收敛\\\Rightarrow\sum_{n=1}^{\infty}a_n收敛，与题设\sum_{n=1}^{\infty}a_n发散矛盾\\\Rightarrow假设不成立，\sum_{n=1}^{\infty}(|a_n|+|b_n|)发散
  $$



# T2

* $$
  \lim_{x\to0^-}g[f(x)]=\lim_{x\to0^-}g(x^2)=\lim_{x\to0^-}2+x^2=2
  $$

* $$
  \lim_{x\to0^+}g[f(x)]=\lim_{x\to0^+}g(-x-1)=\lim_{x\to0^+}3+x=3
  $$

* $$
  \lim_{x\to0^-}g[f(x)]\neq\lim_{x\to0^+}g[f(x)]\\\Rightarrow x=0是g[f(x)]的跳跃间断点
  $$

* 



# T1

* $$
  x>0,\int_{-\infty}^{x}f(t)dt=\int_{-\infty}^{0}e^xdx+\int_{0}^{x}t^2dt=1+\frac{x^3}{3}
  $$

* $$
  \Rightarrow I=\lim_{x\to0^+}(1+\frac{x^3}{3})^{\frac{1}{x(1-cosx)}}\stackrel{1^\infty}=e^A
  $$

* $$
  其中A=\lim_{x\to0^+}\frac{1}{x(1-cosx)}(1+\frac{x^3}{3}-1)=\frac{2}{3}
  $$

* $$
  \Rightarrow I=e^{\frac{2}{3}}
  $$

  
