
$$
k=\lim_{x\to\infty}\frac{y}{x}\ne0 
$$

$$
b=\lim_{x\to\infty}(y-kx)
$$

$$
斜渐近线:y=kx+b
$$

$$
\lim_{x\to\infty}[x(……)-kx]=\lim_{x\to\infty}[x(……-k)],k\ne0
$$


$$
\lim_{x\to\infty}[\ln(……)-1]=\lim_{x\to\infty}[\ln(……)-\ln e]
$$

$$
\lim_{x\to\infty}[\ln(……)-x]=\lim_{x\to\infty}[\ln(……)-\ln e^x]
\\x=\ln e^x=x\ln e
$$

$$
r^2+ar+b=0
$$

$$
\mathrm{b}=\lim _{x \rightarrow \infty}(y-k x)=\lim _{x \rightarrow \infty} \left[x\ln \left(e+\frac{1}{x-1}\right)-x\right]=
\lim _{x \rightarrow \infty} x\left[\ln \left(e+\frac{1}{x-1}\right){-1}\right]=\lim _{x \rightarrow \infty} x\left[\ln \left(e+\frac{1}{x-1}\right)-\ln e\right]=\lim _{x \rightarrow \infty} x \ln \left(1+\frac{1}{e(x-1)}\right)
$$

$$
P\{X=k\}=\frac{e^{-\lambda}\lambda^k}{k!},k=0,1,2,……,\lambda>0
\\P\{X=k\}=\frac{e^{-1}1^k}{k!},k=0,1,2,……,\lambda=1
\\P\{X=k\}=\frac{e^{-1}}{k!},k=0,1,2,……,\lambda=1
\\P\{X=k\}=\frac{e^{-1}}{k!},k=1,2,……,\lambda=1
$$

$$
e^{-1}+\sum_{k=1}^{\infty}(k-1)\frac{e^{-1}}{k!}=e^{-1}+\sum_{k=0}^{\infty}(k-1)\frac{e^{-1}}{k!}+e^{-1}=2e^{-1}+E(X-)
$$

$$
E(X-1)=\sum_{k=0}^{\infty}(k-1)\frac{e^{-1}}{k!}
$$

$$
\begin{array}{l}
e^{x}=1+x+\frac{x^{2}}{2 !}+\frac{x^{3}}{3 !}+\frac{x^{4}}{4 !}+\cdots \cdots+\frac{x^{n}}{n !}+o\left(x^{n}\right) \\
\sin x=x-\frac{x^{3}}{3 !}+\cdots \cdots+\frac{(-1)^{n}}{(2 n+1) !} x^{2 n+1}+o\left(x^{2 n+1}\right) \\
\cos x=1-\frac{x^{2}}{2 !}+\cdots \cdots+\frac{(-1)^{n}}{(2 n) !} x^{2 n}+o\left(x^{2 n}\right) \\
\frac{1}{1-x}=1+x+x^{2}+x^{3}+\cdots \cdots+x^{n}+o\left(x^{n}\right) \\
\frac{1}{1+x}=1-x+x^{2}-x^{3}+\cdots \cdots+(-1)^{n} x^{n}+o\left(x^{n}\right) \\
\ln (1+x)=x-\frac{x^{2}}{2}+\frac{x^{3}}{3}-\cdots \cdots+\frac{(-1)^{n-1}}{n} x^{n}+o\left(x^{n}\right)
\end{array}
$$

$$
e^{-1}+\sum_{k=2}^{\infty}(k-1)\frac{e^{-1}}{k!}=e^{-1}+\sum_{k=2}^{\infty}\frac{e^{-1}}{(k-1)!}-\sum_{k=2}^{\infty}\frac{e^{-1}}{k!}
\\=e^{-1}+e^{-1}\left(\sum_{k=2}^{\infty}\frac{1}{(k-1)!}-\sum_{k=2}^{\infty}\frac{1}{k!}\right)
\\=e^{-1}+e^{-1}[e-1-(e-2)]=\frac{2}{e}
$$

$$
e^{x}=1+x+\frac{x^{2}}{2 !}+\frac{x^{3}}{3 !}+\frac{x^{4}}{4 !}+\cdots \cdots+\frac{x^{n}}{n !}+o\left(x^{n}\right)
\\e^x=\frac{x^0}{0!}+\frac{x^1}{1!}+\frac{x^{2}}{2 !}+\frac{x^{3}}{3 !}+\frac{x^{4}}{4 !}+\cdots \cdots+\frac{x^{n}}{n !}+o\left(x^{n}\right),(x\neq0)\\
e^x=\sum_{k=0}^{\infty}\frac{x^k}{k!},(x\neq0)
\\e=\sum_{k=0}^{\infty}\frac{1}{k!},(x=1)
$$

$$
解: 特征方程  r^{2}+a r+b=0  的特征根记为  r_{1}  和  r_{2} .\\
(1) 若  r_{1} \neq r_{2} , 则  y=C_{1} e^{r_{1} x}+C_{2} e^{r_{2} x}(其中C_1和C_2为任意常数),-\infty<x<+\infty .
\\(2) 若  r_{1}=r_{2}=r , 则  y=\left(C_{1}+C_{2} x\right)e^{rx}(其中C_1和C_2为任意常数),-\infty<x<+\infty .

\\(3) 若  r_{1,2}=\alpha \pm \beta i , 则  y=e^{\alpha x}\left(C_{1} \cos \beta x+C_{2} \sin \beta x\right)(其中C_1和C_2为任意常数),-\infty<x<+\infty .
$$

$$
\begin{cases} 
a^2-4b<0\\
-\frac{a}{2}=0
       \end{cases}
$$

$$
P\{X=0\}=\frac{e^{-1}\cdot1^0}{0!}=\frac{1}{e},\lambda=1
\\=1\cdot P\{X=0\}+\sum_{k=1}^{\infty}(k-1)P\{X=k\}
\\=\frac{1}{e}+\sum_{k=1}^{\infty}(k-1)P\{X=k\}
\\=\frac{1}{e}+\sum_{k=0}^{\infty}(k-1)P\{X=k\}-(0-1)P\{X=0\}
\\=\frac{1}{e}+E(X-1)+P\{X=0\}=\frac{1}{e}+0+\frac{1}{e}=\frac{2}{e}
$$

$$
E\left[f(X)\right]=\sum_{k=x_1}^{x_n} f(k)P\{X=k\}
\\x_1,x_2,……,x_n
$$

$$
\frac{k-1}{k!}=\neq\frac{1}{(k-1)!}
\\\frac{k-1}{k!}=\frac{\cancel{k-1}}{k\cdot\cancel{(k-1)}\cdot(k-2)……\cdot1}=\frac{1}{k\cdot(k-2)……\cdot1}\\
\frac{1}{(k-1)!}=\frac{1}{(k-1)\cdot(k-2)\cdot……\cdot1}
$$

$$
\frac{k}{k!}=\frac{1}{(k-1)!}
\\\frac{k}{k!}=\frac{\cancel{k}}{\cancel{k}\cdot{k-1}\cdot……\cdot1}=\frac{1}{(k-1)\cdot(k-2)……\cdot1}\\
\frac{1}{(k-1)!}=\frac{1}{(k-1)\cdot(k-2)\cdot……\cdot1}
$$


$$
E(X-1)=EX-1=\lambda-1=0\\
E(X-1)=\sum_{k=0}^{\infty}(k-1)P\{X=k\}
$$

$$
e^x=1+x+\frac{x^2}{2!}+\frac{x^3}{3!}+……+\frac{x^n}{n!}+o(x^n)
\\e^x=\sum_{k=0}^{\infty}\frac{x^k}{k!}=\frac{x^0}{0!}+\frac{x^1}{1!}+\frac{x^2}{2!}……,x\neq0
\\e=\sum_{k=0}^{\infty}\frac{1}{k!}=\frac{1}{0!}+\frac{1}{1!}+\frac{1}{2!}+……,x=1\\
1=\frac{x^0}{0!}=1\\
x=\frac{x^1}{1!}=x
$$

$$
\\=1\cdot P\{X=0\}+0\cdot P\{X=1\}+\sum_{k=2}^{\infty}(k-1)P\{X=k\}
\\=1\cdot P\{X=0\}+0\cdot P\{X=1\}+\sum_{k=2}^{\infty}(k-1)\cdot\frac{e^{-1}}{k!}
\\=\frac{1}{e}+\frac{1}{e}\sum_{k=2}^{\infty}\frac{1}{(k-1)!}-\frac{1}{e}\sum_{k=2}^{\infty}\frac{1}{k!}\\
=\frac{1}{e}+\frac{1}{e}\left(\frac{1}{1!}+\frac{1}{2!}+\frac{1}{3!}……\right)-\frac{1}{e}\left(\frac{1}{2!}+\frac{1}{3!}+\frac{1}{4!}……\right)
\\=\frac{1}{e}+\frac{1}{e}\left(e-1\right)-\frac{1}{e}\left(e-2\right)\\=\frac{1}{e}+\left(1-\frac{1}{e}\right)-\left(1-\frac{2}{e}\right)=\frac{2}{e}
$$

$$
P\{X=k\}=\frac{e^{-\lambda}\lambda^k}{k!}=\frac{e^{-1}\cdot1^k}{k!}=\frac{e^{-1}}{k!},k=0,1,2,……,\lambda=1
$$

$$
y=C_1e^{r_1x}+C_2e^{r_2x}(C_1和C_2是任意常数),-\infty<x<+\infty\\
y=(C_1+C_2x)e^{rx}(C_1和C_2是任意常数),-\infty<x<+\infty\\
y=e^{\alpha x}(C_1\cos\beta x+C_2\sin\beta x)(C_1和C_2是任意常数),-\infty<x<+\infty\\
r_{1,2}=\alpha\pm\beta i
$$

$$
\Delta=b^2-4ac=a^2-4b>0
\\\Delta=b^2-4ac=a^2-4b=0
\\\Delta=b^2-4ac=a^2-4b<0
\\\alpha=-\frac{b}{2a}=-\frac{a}{2}
$$

$$
\frac{\lambda-1}{-3}=\frac{3}{\lambda+5}=\frac{-3}{-3}\\
\Rightarrow \lambda=-2
$$

$$
\left(\begin{array}{ll}
1 & -3 & 3\\
3 & -5 & 3\\
6 & -6 &4
\end{array}\right)
$$

$$
\left|\begin{array}{ll}
\lambda-1 & 3 & -3\\
-3 & \lambda+5 & -3\\
-6 & 6 &\lambda-4
\end{array}\right|
$$

$$
\frac{\lambda-1}{-3}=\frac{3}{\lambda5}=\frac{-3}{-3}=1
$$

$$
\lambda=-2
$$

$$
\left|\begin{array}{ll}
\lambda-1+3 & 3-\lambda-5 & -3+3\\
-3 & \lambda+5 & -3\\
-6 & 6 &\lambda-4
\end{array}\right|=\left|\begin{array}{ll}
\lambda+2 & -\lambda-2 & 0\\
-3 & \lambda+5 & -3\\
-6 & 6 &\lambda-4
\end{array}\right|=(\lambda+2)\left|\begin{array}{ll}
1 & -1 & 0\\
-3 & \lambda+5 & -3\\
-6 & 6 &\lambda-4
\end{array}\right|
$$

$$
(\lambda+2)\left|\begin{array}{ll}
1 & -1 & 0\\
-3 & \lambda+5 & -3\\
-6 & 6 &\lambda-4
\end{array}\right|=(\lambda+2)\left|\begin{array}{ll}
1 & -1 & 0\\
-3+3 & \lambda+5-3 & -3\\
-6 & 6 &\lambda-4
\end{array}\right|=(\lambda+2)\left|\begin{array}{ll}
1 & -1 & 0\\
0 & \lambda+2 & -3\\
-6 & 6 &\lambda-4
\end{array}\right|
$$

$$
(\lambda+2)\left|\begin{array}{ll}
1 & -1 & 0\\
0 & \lambda+2 & -3\\
-6 & 6 &\lambda-4
\end{array}\right|=(\lambda+2)\left|\begin{array}{ll}
1 & -1 & 0\\
0 & \lambda+2 & -3\\
-6+6 & 6-6 &\lambda-4
\end{array}\right|=(\lambda+2)\left|\begin{array}{ll}
1 & -1 & 0\\
0 & \lambda+2 & -3\\
0 & 0 &\lambda-4
\end{array}\right|
$$

$$
(\lambda+2)^2\cdot(\lambda-4)=0
$$

$$
\Rightarrow \lambda_{1,2}=-2,\lambda_3=4
$$

$$
\left|\begin{array}{ll}
-2-1 & 3 & -3\\
-3 & -2+5 & -3\\
-6 & 6 &-2-4
\end{array}\right|=\left|\begin{array}{ll}
-3 & 3 & -3\\
-3 & 3 & -3\\
-6 & 6 &-6
\end{array}\right|=0
$$

$$
\left|\begin{array}{ll}
4-1 & 3 & -3\\
-3 & 4+5 & -3\\
-6 & 6 &4-4
\end{array}\right|=\left|\begin{array}{ll}
3 & 3 & -3\\
-3 & 9 & -3\\
-6 & 6 &0
\end{array}\right|=\left|\begin{array}{ll}
3 & 3 & -3\\
-3+3 & 9+3 & -3-3\\
-6+6 & 6+6 &0-6
\end{array}\right|=\left|\begin{array}{ll}
3 & 3 & -3\\
0 & 12 & -6\\
0 & 12 &-6
\end{array}\right|=0
$$

$$
\left(\begin{array}{ll}
2 & 1 & 3\\
4 & 2 & 6\\
6 & 3 & 9
\end{array}\right)
$$

$$
\left|\begin{array}{ll}
\lambda-2 & -1 & -3\\
-4 & \lambda-2 & -6\\
-6 & -3 & \lambda-9
\end{array}\right|
$$

$$
\frac{\lambda-2}{-4}=\frac{-1}{\lambda-2}=\frac{-3}{-6}=\frac{1}{2}
$$

$$
\Rightarrow \lambda_{}=0,\lambda_3=4
$$

$$
\left|\begin{array}{ll}
\lambda-2 & -1 & -3\\
-4 & \lambda-2 & -6\\
-6 & -3 & \lambda-9
\end{array}\right|=\left|\begin{array}{ll}
\lambda-2 & -1 & -3\\
-4-2\lambda+4 & \lambda-2+2 & -6+6\\
-6 & -3 & \lambda-9
\end{array}\right|=\left|\begin{array}{ll}
\lambda-2 & -1 & -3\\
-2\lambda & \lambda & 0\\
-6 & -3 & \lambda-9
\end{array}\right|
\\=\lambda\cdot\left|\begin{array}{ll}
\lambda-2 & -1 & -3\\
-2 & 1 & 0\\
-6 & -3 & \lambda-9
\end{array}\right|=\lambda\cdot\left|\begin{array}{ll}
\lambda-2 & -1 & -3\\
-2 & 1 & 0\\
-6 & -3 & \lambda-9
\end{array}\right|
\\\lambda\cdot\left|\begin{array}{ll}
\lambda-2-2 & -1+1 & -3\\
-2 & 1 & 0\\
-6-6 & -3+3 & \lambda-9
\end{array}\right|=
\lambda\cdot\left|\begin{array}{ll}
\lambda-4 & 0 & -3\\
-2 & 1 & 0\\
-12 & 0 & \lambda-9
\end{array}\right|
=\lambda\cdot1\cdot(-1)^{2+2}\left|\begin{array}{ll}
\lambda-4  & -3\\

-12  & \lambda-9
\end{array}\right|=\lambda\cdot\left|\begin{array}{ll}
\lambda-4  & -3\\

-12  & \lambda-9
\end{array}\right|
\\=\lambda^2(\lambda-13)\Rightarrow\lambda_{1,2}=0,\lambda_3=13
$$

$$
\left(\begin{array}{ll}
1  &   6  & -3\\
-1 &   4  & -3\\
1  &  -2  &  5
\end{array}\right)
$$

$$
\left|\begin{array}{ll}
1  &   6  & -3\\
-1 &   4  & -3\\
1  &  -2  &  5
\end{array}\right|=\left|\begin{array}{ll}
\lambda-1  &   -6  & 3\\
1 &   \lambda-4  & 3\\
-1  &  2  &  \lambda-5
\end{array}\right|
$$

$$
\frac{\lambda-1}{1}=\frac{-6}{\lambda-4}=\frac{3}{3}=1
$$

$$
\Rightarrow\lambda=2\\
\Rightarrow\lambda=-2
$$

$$
\frac{1}{-1}=\frac{\lambda-4}{2}=\frac{3}{\lambda-5}=-1
\\\Rightarrow\lambda=2
$$

$$
\left|\begin{array}{ll}
\lambda-1  &   -6  & 3\\
1 &   \lambda-4  & 3\\
-1  &  2  &  \lambda-5
\end{array}\right|=\left|\begin{array}{ll}
\lambda-1  &   -6  & 3\\
1 &   \lambda-4  & 3\\
-1+1  &  2+\lambda-4  &  \lambda-5+3
\end{array}\right|=\left|\begin{array}{ll}
\lambda-1  &   -6  & 3\\
1 &   \lambda-4  & 3\\
0  &  \lambda-2  &  \lambda-2
\end{array}\right|=(\lambda-2)\cdot\left|\begin{array}{ll}
\lambda-1  &   -6  & 3\\
1 &   \lambda-4  & 3\\
0  &  1  &  1
\end{array}\right|
$$

$$
(\lambda-2)\cdot\left|\begin{array}{ll}
\lambda-1  &   -6  & 3\\
1 &   \lambda-4  & 3\\
0  &  1  &  1
\end{array}\right|=(\lambda-2)\cdot\left|\begin{array}{ll}
\lambda-1  &   -6-3  & 3\\
1 &   \lambda-4-3  & 3\\
0  &  1-1  &  1
\end{array}\right|=(\lambda-2)\cdot\left|\begin{array}{ll}
\lambda-1  &   -9  & 3\\
1 &   \lambda-7  & 3\\
0  &  0  &  1
\end{array}\right|
\\=(\lambda-2)\cdot1\cdot(-1)^{3+3}\left|\begin{array}{ll}
\lambda-1  &   -9 \\
1 &   \lambda-7  \\

\end{array}\right|=(\lambda-2)(\lambda-4)^2=0
$$

$$
\Rightarrow\lambda_1=2,\lambda_{2,3}=4
$$

$$
\left(\begin{array}{ll}
2  &   -1  & 3\\
-1 &   2  & 0\\
3  &  0  &  6
\end{array}\right)
$$

$$
\left|\begin{array}{ll}
\lambda-2  &   1  & -3\\
1 &   \lambda-2  & 0\\
-3  &  0  &  \lambda-6
\end{array}\right|
$$

$$
|A|=\left|\begin{array}{ll}
2  &   -1  & 3\\
-1 &   2  & 0\\
3  &  0  &  6
\end{array}\right|=3\left|\begin{array}{ll}
2  &   -1  & 3\\
-1 &   2  & 0\\
1  &  0  &  2
\end{array}\right|=3\left|\begin{array}{ll}
2  &   -1  & 3-4\\
-1 &   2  & 0+2\\
1  &  0  &  2-2
\end{array}\right|=3\left|\begin{array}{ll}
2  &   -1  & -1\\
-1 &   2  & 2\\
1  &  0  &  0
\end{array}\right|=3\cdot1\cdot(-1)^{3+1}\cdot\left|\begin{array}{ll}
  -1  & -1\\
  2  & 2\\

\end{array}\right|=0
$$

$$
\left|\begin{array}{ll}
\lambda-2  &   1  & -3\\
1+2\lambda-4 &   \lambda-2+2  & 0-6\\
-3  &  0  &  \lambda-6
\end{array}\right|=\left|\begin{array}{ll}
\lambda-2  &   1  & -3\\
2\lambda-3 &   \lambda  & -6\\
-3  &  0  &  \lambda-6
\end{array}\right|=\left|\begin{array}{ll}
\lambda-2  &   1  & -3\\
2\lambda-3+3 &   \lambda  & -6-\lambda+6\\
-3  &  0  &  \lambda-6
\end{array}\right|=\left|\begin{array}{ll}
\lambda-2  &   1  & -3\\
2\lambda &   \lambda  & -\lambda\\
-3  &  0  &  \lambda-6
\end{array}\right|
\\=\lambda\left|\begin{array}{ll}
\lambda-2  &   1  & -3\\
2 &   1  & -1\\
-3  &  0  &  \lambda-6
\end{array}\right|=\lambda\left|\begin{array}{ll}
\lambda-2-2  &   1  & -3+1\\
2-2 &   1  & -1+1\\
-3  &  0  &  \lambda-6
\end{array}\right|=\lambda\left|\begin{array}{ll}
\lambda-4  &   1  & -2\\
0 &   1  & 0\\
-3  &  0  &  \lambda-6
\end{array}\right|=\lambda\left|\begin{array}{ll}
\lambda-4 & -2\\

-3 &  \lambda-6
\end{array}\right|=\lambda\left|\begin{array}{ll}
\lambda-4 & -2\\

-3 &  \lambda-6
\end{array}\right|
\\\lambda(\lambda^2-10\lambda+24-6)=\lambda(\lambda^2-10\lambda+18)=0
\\\Rightarrow\lambda_1=0,\lambda_2=5+\sqrt7,\lambda_2=5-\sqrt7
$$

$$
A\left(\begin{array}{ll}
1\\
1\\
1
\end{array}\right)=2\left(\begin{array}{ll}
1\\
1\\
1
\end{array}\right)\Rightarrow\lambda=2
$$

$$
A=\left(\begin{array}{ll}
1  &   -1  & 1\\
0 &   1  & 1\\
1  &  0  &  2
\end{array}\right)
$$


$$
|\lambda E-A|=\left|\begin{array}{ll}
\lambda-1  & 1  & -1\\
0 &   \lambda-1  & -1\\
-1  &  0  &  \lambda-2
\end{array}\right|
$$

$$
(\lambda-1)^2(\lambda-2)+1-(\lambda-1)=(\lambda^2-2\lambda+1)(\lambda-2)+1-\lambda+1=(\lambda^3-2\lambda^2+\lambda-2\lambda^2+4\lambda-2)-\lambda+2
\\=\lambda^3-4\lambda^2+4\lambda=\lambda(\lambda^2-4\lambda+4)=\lambda(\lambda-2)^2
$$

$$
\lambda_1=0,\lambda_{2,3}=2
$$

$$
A=\left(\begin{array}{ll}
1  &   2  & -3\\
-1 &   4  & -3\\
1  &  -2  &  5
\end{array}\right)
$$

$$
\left|\begin{array}{ll}
\lambda-1  &   -2  & 3\\
1 &   \lambda-4  & 3\\
-1  &  2  &  \lambda-5
\end{array}\right|
$$

$$
\frac{\lambda-1}{1}=\frac{-2}{\lambda-4}=\frac{3}{3}=1
\\\Rightarrow\lambda=2
$$

$$
\left|\begin{array}{ll}
\lambda-1-1  &   -2-\lambda+4  & 3-3\\
1 &   \lambda-4  & 3\\
-1  &  2  &  \lambda-5
\end{array}\right|=\left|\begin{array}{ll}
\lambda-2  &   -\lambda+2  & 0\\
1 &   \lambda-4  & 3\\
-1  &  2  &  \lambda-5
\end{array}\right|=(\lambda-2)\left|\begin{array}{ll}
1  &   -1  & 0\\
1 &   \lambda-4  & 3\\
-1  &  2  &  \lambda-5
\end{array}\right|
$$

$$
(\lambda-2)\left|\begin{array}{ll}
1  &   -1  & 0\\
1 &   \lambda-4  & 3\\
-1  &  2  &  \lambda-5
\end{array}\right|=(\lambda-2)\left|\begin{array}{ll}
1-1  &   -1  & 0\\
1+\lambda-4 &   \lambda-4  & 3\\
-1+2  &  2  &  \lambda-5
\end{array}\right|=(\lambda-2)\left|\begin{array}{ll}
0  &   -1  & 0\\
\lambda-3 &   \lambda-4  & 3\\
1  &  2  &  \lambda-5
\end{array}\right|
$$

$$
(\lambda-2)\cdot\left|\begin{array}{ll}
0  &   -1  & 0\\
\lambda-3 &   \lambda-4  & 3\\
1  &  2  &  \lambda-5
\end{array}\right|=(\lambda-2)\cdot(-1)\cdot(-1)^{1+2}\cdot\left|\begin{array}{ll}
\lambda-3   & 3\\
1    &  \lambda-5
\end{array}\right|=(\lambda-2)\cdot[(\lambda-3)(\lambda-5)-3]
\\=(\lambda-2)\cdot[(\lambda-3)(\lambda-5)-3]=(\lambda-2)\cdot[\lambda^2-8\lambda+15-3]=(\lambda-2)\cdot[\lambda^2-8\lambda+12]=(\lambda-2)^2(\lambda-6)
$$

$$
\Rightarrow\lambda_{1,2}=2,\lambda_3=6
$$

$$
|\lambda E-A|=\left|\begin{array}{ll}
\lambda-1  & 1  & -1\\
0 &   \lambda-1  & -1\\
-1  &  0  &  \lambda-2
\end{array}\right|=\left|\begin{array}{ll}
\lambda-1+1  & 1+\lambda-1  & -1-\lambda+2-1\\
0 &   \lambda-1  & -1\\
-1  &  0  &  \lambda-2
\end{array}\right|
\\=\left|\begin{array}{ll}
\lambda  & \lambda  & -\lambda\\
0 &   \lambda-1  & -1\\
-1  &  0  &  \lambda-2
\end{array}\right|=\lambda\cdot\left|\begin{array}{ll}
1  & 1  & -1\\
0 &   \lambda-1  & -1\\
-1  &  0  &  \lambda-2
\end{array}\right|=\lambda\cdot\left|\begin{array}{ll}
1  & 0  & 0\\
0 &   \lambda-1  & -1\\
-1  &  1  &  \lambda-3
\end{array}\right|=\lambda\cdot\left|\begin{array}{ll}

 \lambda-1  & -1\\
 1  &  \lambda-3
\end{array}\right|\\=\lambda\cdot(\lambda-4\lambda+4)=\lambda(\lambda-2)^2
$$

$$
\left|\begin{array}{ll}
\lambda-1  &   -2  & 3\\
1 &   \lambda-4  & 3\\
-1  &  2  &  \lambda-5
\end{array}\right|=(\lambda-1)(\lambda-4)(\lambda-5)+6+6+3(\lambda-4)+2(\lambda-5)-6(\lambda-1)
$$

$$
A=\left(\begin{array}{ll}
2  &   -1  & 2\\
5 &   -3  & 3\\
-1  &  0  &  -2
\end{array}\right)
$$

$$
\left|\begin{array}{ll}
\lambda-2  &   1  & -2\\
-5 &   \lambda+3  & -3\\
1  &  0  &  \lambda+2
\end{array}\right|
$$

$$
\frac{\lambda-2}{-5}=\frac{1}{\lambda+3}=\frac{-2}{-3}=\frac{2}{3}
$$

$$
\frac{\lambda-2}{-5}=\frac{2}{3}\Rightarrow\lambda=-\frac{4}{3}
$$

$$
\frac{1}{\lambda+3}=\frac{2}{3}\Rightarrow\lambda=-\frac{3}{2}
$$

$$
(\lambda-2)(\lambda+3)(\lambda+2)-3+2(\lambda+3)+5(\lambda+2)
$$

$$
\lambda_{1,2,3}=-1
$$

$$
\iff
$$

$$
\exist
$$

$$
(-1)^{\frac{n(n-1)}{2}}
$$

$$
(-1)^{\frac{2(2-1)}{2}}
$$

$$
|\lambda E-A|=\left|\begin{array}{ll}
\lambda    & 1\\
-1  &  \lambda
\end{array}\right|=\lambda^2+1=0
$$

$$
\lambda_{1,2}=2
$$

$$
(AB)^T=B^TA^T
$$

$$
(\lambda A)^T=\lambda A^T
$$

$$
A^T=A^{-1}
$$

$$
A=\left(\begin{array}{ll}
1  &   2  &3\\
2 &   3  & 4\\
3  &  5  &  7
\end{array}\right)
$$

$$
A\left(\begin{array}{ll}
1 \\
1 \\
1
\end{array}\right)=2\left(\begin{array}{ll}
1 \\
1 \\
1
\end{array}\right)
$$

$$
A\left(\begin{array}{ll}
1 \\
1 \\
1
\end{array}\right)=\left(\begin{array}{ll}
2 \\
2 \\
2
\end{array}\right)
$$

$$
\alpha=(x,y,1)^T
$$

$$
\left(\begin{array}{ll}
1  &   2  &3\\
2 &   4  & 6\\
3  &  6  &  9
\end{array}\right)
$$

$$
\left(\begin{array}{ll}
1  &   2  &3\\
0 &   0  & 0\\
0  &  0  &  0
\end{array}\right)
$$

$$
令\alpha_1=(x,1,0)^T,\alpha_2=(x,0,1)^T
$$

$$
\alpha_1=(-2,1,0)^T,\alpha_2=(-3,0,1)^T
$$

$$
\alpha_1=(-2,1,0),\alpha_2=(-3,-6,5)^T
$$

$$
\beta_1=\alpha_1=(-2,1,0)^T
\\\beta_2=\alpha_2-\frac{(\alpha_2,\beta_1)}{(\beta_1,\beta_1)}\beta_1=(-3,0,1)^T-\frac{6}{5}(-2,1,0)^T=(-\frac{3}{5},-\frac{6}{5},0)
$$

$$
A=\left(\begin{array}{ll}
2  &  2  &-2\\
2 &   5  & -4\\
-2  &  -4  &  5
\end{array}\right)
$$

$$
AA^T=A^TA=E
$$

$$
E^T=E
$$

$$
E^TE=EE^T=EE=E
$$

$$
\left(\begin{array}{ll}
1 \\
1 \\
1
\end{array}\right)
$$

$$
k_1\left(\begin{array}{ll}
1 \\
0 \\
0
\end{array}\right)+k_2\left(\begin{array}{ll}
0 \\
1 \\
0
\end{array}\right)+k_3\left(\begin{array}{ll}
0 \\
0 \\
1
\end{array}\right)=0
$$

$$
A\sim\Lambda\iff
$$

$$
P^{-1}AP=\Lambda
$$

$$
A\sim\left(\begin{array}{ll}
1  &  0  &0\\
0 &   3  & 0\\
0  &  0  &  5
\end{array}\right)
$$

$$
A=\left(\begin{array}{ll}
0  &  2  &-3\\
-1 &   3  & -3\\
1  &  -2  &  4
\end{array}\right)
$$

$$
\left|\begin{array}{ll}
\lambda  &  -2  &3\\
1 &   \lambda-3  & 3\\
-1  &  2  &  \lambda-4
\end{array}\right|
$$

$$
\frac{\lambda}{1}=\frac{-2}{\lambda-3}=\frac{3}{3}=1\Rightarrow\lambda_1=1
$$

$$
\left|\begin{array}{ll}
\lambda-1  &  -\lambda+1  &0\\
1 &   \lambda-3  & 3\\
-1  &  2  &  \lambda-4
\end{array}\right|=(\lambda-1)\left|\begin{array}{ll}
1  &  -1  &0\\
1 &   \lambda-3  & 3\\
-1  &  2  &  \lambda-4
\end{array}\right|=(\lambda-1)\left|\begin{array}{ll}
1  &  0  &0\\
1 &   \lambda-2  & 3\\
-1  &  1  &  \lambda-4
\end{array}\right|=(\lambda-1)^2(\lambda-5)
$$

$$
\lambda_{1,2}=1,\lambda_3=5
$$

$$
\left(\begin{array}{ll}
1  &  -2  &3\\
1 &   -2  & 3\\
-1  &  2  &  -3
\end{array}\right)\to\left(\begin{array}{ll}
1  &  -2  &3\\
0 &   0  & 0\\
0  &  0  &  0
\end{array}\right)
$$

$$
P^{-1}AP=\Lambda
$$

$$
\alpha=(0,0,1)^T
$$

$$
\alpha_1=(x,0,1)^T,\alpha_2=(x,1,0)^T
$$

$$
\begin{cases}
x_1 + x_2 -3x_4-x_5=0 \\
x_1 - x_2 +2x_3-x_4=0 \\
4x_1 - 2x_2 +6x_3+3x_4-4x_5=0\\
2x_1 +4x_2 -2x_3+4x_4-7x_5=0
\end{cases}
$$

$$
\left\{\begin{array}{l}
a_{11} x_{1}+a_{12} x_{2}+\cdots+a_{1 n} x_{n}=0 \\
a_{21} x_{1}+a_{22} x_{2}+\cdots+a_{2 n} x_{n}=0 \\
\quad\quad\quad\quad\quad\quad\quad……\\
a_{m 1} {x}_{1}+ {a}_{m 2} {x}_{2}+\cdots+a_{m n} x_{n}=0
\end{array}\right.
$$

$$
\Rightarrow
$$

$$
P^{-1}AP=B
$$

$$
B(P^{-1}\alpha)=\lambda(P^{-1}\alpha)
$$

$$
A(P\alpha)=\lambda(P\alpha)
$$

$$
=(\lambda-4)\left|\begin{array}{ll}
1  &  0  &-1\\
-1 &   \lambda+2  & -2\\
3  &  -1  &  \lambda-3
\end{array}\right|=(\lambda-4)\left|\begin{array}{ll}
1  &  0  &0\\
-1 &   \lambda+2  & -3\\
3  &  -1  &  \lambda
\end{array}\right|=(\lambda-4)()
$$

$$
\left(\begin{array}{ll}
0  &  -1  &1\\
-1 &   3  & -2\\
3  &  -1  &  -2
\end{array}\right)\to\left(\begin{array}{ll}
0  &  -1  &1\\
-1 &   3  & -2\\
0  &  0  &  0
\end{array}\right)\to\left(\begin{array}{ll}
-1 &   3  & -2\\
0  &  -1  &1\\
0  &  0  &  0
\end{array}\right)
$$

$$
\left(\begin{array}{ll}
-1 &   3  & -2\\
0  &  -1  &1\\
0  &  0  &  0
\end{array}\right)\to\left(\begin{array}{ll}
1 &   -3  & 2\\
0  &  1  &-1\\
0  &  0  &  0
\end{array}\right)
$$

$$
\left(\begin{array}{ll}
1 &   0  & -1\\
0  &  1  &-1\\
0  &  0  &  0
\end{array}\right)
$$

$$
\alpha_1=(1,1,1)^T
$$

$$
\to\left(\begin{array}{ll}
3  &  -1  &1\\
-1 &   6  & -2\\
3  &  -1  &  1
\end{array}\right)\to\left(\begin{array}{ll}
3  &  -1  &1\\
-1 &   6  & -2\\
0  &  0 &  0
\end{array}\right)
$$

$$
\left(\begin{array}{ll}
3  &  -1  &1\\
-1 &   6  & -2\\
0  &  0 &  0
\end{array}\right)\to\left(\begin{array}{ll}
3  &  -1  &1\\
1 &   -6  & 2\\
0  &  0 &  0
\end{array}\right)
$$

$$
\left(\begin{array}{ll}
3  &  -1  &1\\
1 &   -6  & 2\\
0  &  0 &  0
\end{array}\right)\to\left(\begin{array}{ll}
0  &  17  &-5\\
1 &   -6  & 2\\
0  &  0 &  0
\end{array}\right)\to\left(\begin{array}{ll}
1 &   -6  & 2\\
0  &  17  &-5\\
0  &  0 &  0
\end{array}\right)
$$

$$
\alpha_2=(-4,5,17)^T
$$

$$
\to\left(\begin{array}{ll}
-4 &  -1  &1\\
-1 &   -1  & -2\\
3  &  -1  &  -6
\end{array}\right)\to\left(\begin{array}{ll}
-1 &   -1  & -2\\
3  &  -1  &  -6\\
0  &  0  &  0
\end{array}\right)
$$

$$
\left(\begin{array}{ll}
-1 &   -1  & -2\\
3  &  -1  &  -6\\
0  &  0  &  0
\end{array}\right)\to\left(\begin{array}{ll}
1 &   1  & 2\\
3  &  -1  &  -6\\
0  &  0  &  0
\end{array}\right)\to
$$

$$
\left(\begin{array}{ll}
1 &   1  & 2\\
3  &  -1  &  -6\\
0  &  0  &  0
\end{array}\right)\to\left(\begin{array}{ll}
1 &   1  & 2\\
0  &  -4  &  -12\\
0  &  0  &  0
\end{array}\right)\to\left(\begin{array}{ll}
1 &   1  & 2\\
0  &  1  &  3\\
0  &  0  &  0
\end{array}\right)\to\left(\begin{array}{ll}
1 &   0  & -1\\
0  &  1  &  3\\
0  &  0  &  0
\end{array}\right)
$$

$$
\alpha_3=(1,-3,1)^T
$$

$$
\left(\begin{array}{ll}
0 &   -2  & -4\\
0  &  -2&  -5\\
0  &  0  &  -5
\end{array}\right)\to\left(\begin{array}{ll}
0 &   -2  & -4\\
0  &  0 &0\\
0  &  0  &  -5
\end{array}\right)\to\left(\begin{array}{ll}
0 &   -2  & -4\\
0  &  0  &  -5\\
0  &  0 &0\\
\end{array}\right)
$$

$$
\left(\begin{array}{ll}
0 &   -2  & -4\\
0  &  0  &  -5\\
0  &  0 &0\\
\end{array}\right)\to\left(\begin{array}{ll}
0 &   1  & 2\\
0  &  0  &  5\\
0  &  0 &0\\
\end{array}\right)\to\left(\begin{array}{ll}
0 &   1  & 0\\
0  &  0  &  1\\
0  &  0 &0\\
\end{array}\right)
$$

$$
\alpha_1=(1,0,0)^T
$$

$$
\begin{cases}
x_2=0 \\
x_3=0 \\

\end{cases}
$$

$$
\left(\begin{array}{ll}
2 &   -2  & -4\\
0  &  0  &  -5\\
0  &  0 &-3\\
\end{array}\right)\to\left(\begin{array}{ll}
1 &   -1  & -2\\
0  &  0  &  1\\
0  &  0 &0\\
\end{array}\right)\to\left(\begin{array}{ll}
1 &   -1  & 0\\
0  &  0  &  1\\
0  &  0 &0\\
\end{array}\right)
$$

$$
\alpha_2=(1,1,0)^T
$$

$$
\left(\begin{array}{ll}
5 &   -2  & -4\\
0  &  3  &  -5\\
0  &  0 &0\\
\end{array}\right)
$$

$$
\alpha_3=(\frac{22}{5},5,3)^T
$$

$$
\alpha^ T\beta,\beta^ T\alpha
$$

$$
\beta\alpha^ T,\alpha\beta^ T
$$

$$
tr(\beta\alpha^ T)=tr(\alpha\beta^ T)
$$

$$
\left(\begin{array}{ll}
a_1&
a_2&
a_3&
\cdots&
a_n
\end{array}\right)\left(\begin{array}{ll}
b_1\\
b_2\\
b_3\\
\vdots\\
b_n
\end{array}\right)=a_1b_1+a_2b_2+……+a_nb_n
$$

$$
\left(\begin{array}{ll}
a_1\\
a_2\\
a_3\\
\vdots\\
a_n
\end{array}\right)\left(\begin{array}{ll}
b_1&
b_2&
b_3&
\cdots&
b_n
\end{array}\right)=\left(\begin{array}{ll}
a_1b_1&a_1b_2&\cdots&a_1b_n\\
a_2b_1&a_2b_2&\cdots&a_2b_n\\
a_3b_1&a_3b_2&\cdots&a_3b_n\\
\vdots&\vdots&\cdots&\vdots\\
a_nb_1&a_nb_2&\cdots&a_nb_n
\end{array}\right)
$$

$$
A^n=tr(A)^{n-1}A
$$

$$
A=\alpha\beta^ T,A^{100}=\alpha(\beta^ T\alpha)(\beta^ T\alpha)……(\beta^ T\alpha)\beta^ T=α(\beta^ T\alpha)^{99}\beta^T=[tr(A)]^{99}\alpha\beta^T=[tr(A)]^{99}\cdot A
$$

$$
\left(\begin{array}{ll}
1 &   2  & 3\\
1  &  2  & 3\\
-1  &  -2 &-3\\
\end{array}\right)=\left(\begin{array}{ll}
1\\
1\\
1\\
\end{array}\right)(1 &2 &3)=\alpha\beta^T(\alpha\ne0,\beta\ne0)
$$

$$
\left(\begin{array}{ll}
0 &   0  & 1\\
0  &  0  & 1\\
0  & 0 &1\\
\end{array}\right)=\left(\begin{array}{ll}
1\\
1\\
1\\
\end{array}\right)(0 &0 &1)
$$

$$
\alpha_1=\left(\begin{array}{ll}
1,
2,
3
\end{array}\right)^T
$$

$$
\left(\begin{array}{ll}
1 &   2  & 3\\
0 &  0  & 0\\
0  &  0 &0\\
\end{array}\right)
$$

$$
\alpha_2=(-3,0,1)^T
$$

$$
\alpha_3=(1,-5,3)^T
$$

$$
\sqrt{1^2+2^2+3^2}=\sqrt{1+4+9}=\sqrt{14}\\
\sqrt{(-3)^2+0^2+1^2}=\sqrt{1+9}=\sqrt{10}\\
\sqrt{1^2+(-5)^2+3^2}=\sqrt{1+25+9}=\sqrt{35}\\
$$

$$
\left(\begin{array}{ll}
\frac{1}{\sqrt{14}}&   \frac{-3}{\sqrt{10}}  & \frac{1}{\sqrt{35}}\\
\sqrt{\frac{2}{7}} &  0  & -\sqrt{\frac{5}{7}}\\
\frac{3}{\sqrt{14}} &  \frac{1}{\sqrt{10}} &\frac{3}{\sqrt{35}}\\
\end{array}\right)
$$

$$
\frac{2}{\sqrt{14}}=\sqrt{\frac{4}{14}}=\sqrt{\frac{2}{7}}\\
\frac{-5}{\sqrt{35}}=-\sqrt{\frac{25}{35}}=-\sqrt{\frac{5}{7}}
$$

$$
\alpha_1=(b,b,……,b)^T
$$

$$
A=\left(\begin{array}{ll}
a&b&\cdots&b\\
b&a&\cdots&b\\

\vdots&\vdots&\cdots&\vdots\\
b&b&\cdots&a
\end{array}\right)=\left(\begin{array}{ll}
b&b&\cdots&b\\
b&b&\cdots&b\\

\vdots&\vdots&\cdots&\vdots\\
b&b&\cdots&b
\end{array}\right)+(a-b)E=B+(a-b)E
$$

$$
A=\left(\begin{array}{ll}
0&0&\cdots&0\\
0&0&\cdots&0\\

\vdots&\vdots&\cdots&\vdots\\
0&0&\cdots&0
\end{array}\right)_{n\times n}\Rightarrow\lambda_A=0,0,……，0
$$

$$
E\alpha=\lambda\alpha\Rightarrow\alpha=\lambda\alpha\Rightarrow\lambda=1
$$ {E}

$$
A=E_{n\times n}=\left(\begin{array}{ll}
1&0&\cdots&0\\
0&1&\cdots&0\\

\vdots&\vdots&\cdots&\vdots\\
0&0&\cdots&1
\end{array}\right)_{n\times n}\Rightarrow\lambda_A=1,1,……，1
$$

$$
\lambda_1=\lambda_2=……=\lambda_n=0
$$

$$
A=\left(\begin{array}{ll}
0&b&\cdots&b\\
b&0&\cdots&b\\

\vdots&\vdots&\cdots&\vdots\\
b&b&\cdots&0
\end{array}\right)=\left(\begin{array}{ll}
b&b&\cdots&b\\
b&b&\cdots&b\\

\vdots&\vdots&\cdots&\vdots\\
b&b&\cdots&b
\end{array}\right)+(0-b)E=B-bE
$$

$$
\lambda_1=\lambda_2=……=\lambda_{n-1}=0;\lambda_n=nb
$$

$$
\left(\begin{array}{ll}
b&b&\cdots&b\\
0&0&\cdots&0\\

\vdots&\vdots&\cdots&\vdots\\
0&0&\cdots&0
\end{array}\right)\to\left(\begin{array}{ll}
1&1&\cdots&1\\
0&0&\cdots&0\\

\vdots&\vdots&\cdots&\vdots\\
0&0&\cdots&0
\end{array}\right)
$$

$$
\alpha_1=(-1,1,0,……,0)^T,\alpha_2=(-1,0,1,……,0)^T,……,\alpha_{n-1}=(-1,0,0,……,1)^T
$$

$$
\alpha_n=\frac{1}{b}(b,b,……,b)^T=(1,1,……,1)^T
$$

$$
A\alpha=(B-bE)\alpha=(\lambda-b)\alpha
$$


$$
\lambda_A=\lambda_1=\lambda_2=……=\lambda_n=-b
$$

$$
A=\left(\begin{array}{ll}
a&0&\cdots&0\\
0&a&\cdots&0\\

\vdots&\vdots&\cdots&\vdots\\
0&0&\cdots&a
\end{array}\right)_{n\times n},a
\ne0
$$

$$
λ_1=λ_2=……=λ_n=1
$$

$$
A\alpha=[B+(a-b)E]\alpha=(\lambda+a-b)\alpha
$$

$$
A=\left(\begin{array}{ll}
1&b&\cdots&b\\
b&1&\cdots&b\\

\vdots&\vdots&\cdots&\vdots\\
b&b&\cdots&1
\end{array}\right)=\left(\begin{array}{ll}
b&b&\cdots&b\\
b&b&\cdots&b\\

\vdots&\vdots&\cdots&\vdots\\
b&b&\cdots&b
\end{array}\right)+(1-b)E=B+(1-b)E
$$

$$
\alpha_1=(-3,0,1)^T,\alpha_2=(2,1,0)^T
$$

$$
\left(\begin{array}{ll}
5 &   -2  & 3\\
1 &  2  & 3\\
-1  &  2 &1\\
\end{array}\right)\to\left(\begin{array}{ll}
0 &   0  & 0\\
1 &  2  & 3\\
-1  &  2 &1\\
\end{array}\right)
\to\left(\begin{array}{ll}
1 &  2  & 3\\
0  &  4 &4\\
0 &   0  & 0\\
\end{array}\right)\to\left(\begin{array}{ll}
1 &  2  & 3\\
0  &  1 &1\\
0 &   0  & 0\\
\end{array}\right)
\to\left(\begin{array}{ll}
1 &  0  & 1\\
0  &  1 &1\\
0 &   0  & 0\\
\end{array}\right)
$$

$$
\alpha=(-1,-1,1)^T
$$

$$
P=\left(\begin{array}{ll}
-3 &   2  & -1\\
0 &  1  & -1\\
1  &  0 &1\\
\end{array}\right)
$$

$$
\Lambda=\left(\begin{array}{ll}
1 &     & \\
 &  1  & \\
  &   &5\\
\end{array}\right)
$$

$$
\left(\begin{array}{ll}
0 &   -2  & -1\\
0 &  0  & 0\\
0 &  0 &-2\\
\end{array}\right)\to\left(\begin{array}{ll}
0 &   -2  & -1\\
0 &  0  & 1\\
0 &  0 &0\\
\end{array}\right)\to\left(\begin{array}{ll}
0 &   1  & 0\\
0 &  0  & 1\\
0 &  0 &0\\
\end{array}\right)
$$

$$
\left(\begin{array}{ll}
1 &   -1  & -a\\
0 &  0  & -2\\
0  &  0 &0\\
\end{array}\right)\to\left(\begin{array}{ll}
1 &   -1  & -a\\
0 &  0  & 1\\
0  &  0 &0\\
\end{array}\right)
\to\left(\begin{array}{ll}
1 &   -1  & 0\\
0 &  0  & 1\\
0  &  0 &0\\
\end{array}\right)
$$

$$
A=\left(\begin{array}{ll}
1 &   1  & 0 & 3 &-1\\
0 &  2  & 1&4&1\\
1  &  3 &1 &4&6\\
\end{array}\right)\to\left(\begin{array}{ll}
1 &   1  & 0 & 3 &-1\\
0 &  2  & 1&4&1\\
0  &  2 &1 &1&7\\
\end{array}\right)\to\left(\begin{array}{ll}
1 &   1  & 0 & 3 &-1\\
0 &  2  & 1&4&1\\
0  &  0 &0 &-3&6\\
\end{array}\right)
$$

$$
\left(\begin{array}{ll}
1 &   1  & 0 & 3 &-1\\
0 &  2  & 1&4&1\\
0  &  0 &0 &-3&6\\
\end{array}\right)\to\left(\begin{array}{ll}
1 &   1  & 0 & 3 &-1\\
0 &  2  & 1&4&1\\
0  &  0 &0 &1&-2\\
\end{array}\right)
$$

$$
\left(\begin{array}{ll}
1 &   1  & 0 & 3 &-1\\
0 &  2  & 1&4&1\\
0  &  0 &0 &1&-2\\
\end{array}\right)\to\left(\begin{array}{ll}
1 &   1  & 0 & 3 &-1\\
0 &  2  & 1&4&1\\
0  &  0 &0 &1&-2\\
\end{array}\right)
$$

$$
\left(\begin{array}{ll}
1 &   1  & 0 & 3 &-1\\
0 &  2  & 1&4&1\\
0  &  0 &0 &1&-2\\
\end{array}\right)\to\left(\begin{array}{ll}
1 &   1  & 0 & 0 &5\\
0 &  2  & 1&0&9\\
0  &  0 &0 &1&-2\\
\end{array}\right)
$$

$$
\alpha_1=(-5,0,-9,2,1)^T\\
\alpha_2=(-1,1,-2,0,0)^T
$$

$$
\left(\begin{array}{ll}
1 &   1  & 0 & 0 &5\\
0 &  2  & 1&0&9\\
0  &  0 &0 &1&-2\\
\end{array}\right)\to\left(\begin{array}{ll}
1 &   1  & 0 & 0 &5\\
0 &  1  & \frac{1}{2}&0&\frac{9}{2}\\
0  &  0 &0 &1&-2\\
\end{array}\right)
$$

$$
\left(\begin{array}{ll}
1 &   1  & 0 & 0 &5\\
0 &  1  & \frac{1}{2}&0&\frac{9}{2}\\
0  &  0 &0 &1&-2\\
\end{array}\right)\to\left(\begin{array}{ll}
1 &   0  &- \frac{1}{2} & 0 &\frac{1}{2}\\
0 &  1  & \frac{1}{2}&0&\frac{9}{2}\\
0  &  0 &0 &1&-2\\
\end{array}\right)
$$

$$
\left(\begin{array}{ll}
1 &   1  & 0 & 3 &-1\\
0 &  2  & 1&4&1\\
0  &  0 &0 &1&-2\\
\end{array}\right)\to\left(\begin{array}{ll}
1 &   1  & 0 & 3 &-1\\
0 &  1  & \frac{1}{2}&2&\frac{1}{2}\\
0  &  0 &0 &1&-2\\
\end{array}\right)
$$

$$
\left(\begin{array}{ll}
1 &   1  & 0 & 3 &-1\\
0 &  1  & \frac{1}{2}&2&\frac{1}{2}\\
0  &  0 &0 &1&-2\\
\end{array}\right)\to\left(\begin{array}{ll}
1 &   0  & -\frac{1}{2} & 1 &-\frac{3}{2}\\
0 &  1  & \frac{1}{2}&2&\frac{1}{2}\\
0  &  0 &0 &1&-2\\
\end{array}\right)
$$

$$
\left(\begin{array}{ll}
1 &   0  & -\frac{1}{2} & 1 &-\frac{3}{2}\\
0 &  1  & \frac{1}{2}&2&\frac{1}{2}\\
0  &  0 &0 &1&-2\\
\end{array}\right)\to\left(\begin{array}{ll}
1 &   0  & -\frac{1}{2} & 0 &\frac{1}{2}\\
0 &  1  & \frac{1}{2}&0&\frac{9}{2}\\
0  &  0 &0 &1&-2\\
\end{array}\right)
$$

$$
\alpha_1=(-\frac{1}{2},-\frac{9}{2},0,2,1)^T\\
\alpha_2=(\frac{1}{2},-\frac{1}{2},1,0,0)^T
$$

$$
\overline X =\frac{各样本值之和}{容量} 
\\S^2=\frac{(各样本值-样本均值)的平方之和}{容量-1}
$$

$$
S^2=\frac{(各样本值平方之和-容量×样本均值的平方)}{容量-1}=\frac{\sum_{i=1}^{n}X_i^2-n\overline X^2}{n-1}
$$

$$
\overline X =\frac{1}{n}\sum_{i=1}^nX_i=A_1=\frac{1}{n}\sum_{i=1}^nX_i^1
$$

$$
S^2=\frac{\sum_{i=1}^n(X_i-\overline X)^2}{n-1}\ne B_2=\frac{\sum_{i=1}^n(X_i-\overline X)^2}{n}
$$

$$
A_2=\frac{1}{n}\sum_{i=1}^nX_i^2
$$

$$
\ne B_2=\frac{1}{n}\sum_{i=1}^n(X_i-\overline X )^2
$$

$$
E\overline X=E(\frac{1}{n}\sum_{i=1}^nX_i)=\frac{n\mu}{n}=\mu
$$

$$
D\overline X=D(\frac{1}{n}\sum_{i=1}^nX_i)
$$

$$
D(\frac{1}{n}\sum_{i=1}^nX_i)=\frac{1}{n^2}D(\sum_{i=1}^nX_i)=\frac{n\sigma^2}{n^2}=\frac{\sigma^2}{n}
$$

$$
f(x)=\frac{1}{\sqrt{2 \pi} \sigma} \mathrm{e}^{-\frac{1}{2}\left(\frac{x-\mu}{\sigma}\right)^{2}}=\frac{1}{\sqrt{2 \pi} \sigma} \mathrm{e}^{-\frac{({x-\mu})^2}{2{\sigma}^{2}}},(-\infty<x<+\infty)
$$

$$
\Rightarrow
$$

$$
\overline X=\frac{1}{n}\sum_{i=1}^{n}X_i
$$

$$
S^2=\frac{1}{n-1}\sum_{i=1}^n(X_i-\overline X)^2=\frac{1}{n-1}(\sum_{i=1}^nX_i^2- n\overline X^2)
$$

$$
\overline X\sim N(\mu,\frac{\sigma^2}{n})
$$

$$
\frac {\overline X-\mu}{\sigma/\sqrt n}=\frac{\sqrt n(\overline X-\mu)}{\sigma}\sim N(0,1)
$$

$$
\frac{1}{\sigma^2}\sum_{i=1}^n(X_i-\mu)^2\sim\chi^2(n)
$$

$$
\frac{(n-1)S^2}{\sigma^2}=\sum_{i=1}^{n}(\frac{X_i-\overline X}{\sigma})^2\sim\chi^2(n-1)
$$

$$
\frac{n(\overline X-\mu)^2}{S^2}\sim F(1,n-1)
$$

$$
X_i\stackrel{iid}{\sim}N(\mu,\sigma^2)
$$

$$
\frac{X_i-\mu}{\sigma}\sim N(0,1)
$$

$$
\sum_{i=1}^{n}\left(\frac{X_i-\mu}{\sigma}\right)^2\sim \chi^2(n)
$$

$$
\frac{1}{\sigma^2}\sum_{i=1}^{n}\left({X_i-\mu}\right)^2\sim \chi^2(n)
$$

$$
\frac{(n-1)S^2}{\sigma^2}
$$

$$
\frac{\overline X-\mu}{S/\sqrt n}\sim t(n-1)
$$

$$
t=\frac{\frac {\overline X-\mu}{\sigma/\sqrt n}}{\sqrt{\frac{(n-1)S^2}{\sigma^2}/(n-1)}}=\frac{\overline X-\mu}{S/\sqrt n}\sim t(n-1)
$$

$$
t=\frac{X}{\sqrt {Y/(n-1)}}\sim t(n-1)
$$

$$
t^2=\frac{X^2/1}{Y/(n-1)}\sim F(1,n-1)
$$

$$
\frac{(n-1)S^2}{\sigma^2}\sim\chi^2(n-1)
$$


$$
X_i\stackrel{iid}{\sim}N(\mu_1,\sigma^2)\\
Y_i\stackrel{iid}{\sim}N(\mu_2,2\sigma^2)
$$

$$
\frac{(n-1)S_1^2}{\sigma^2}\sim\chi^2(n-1)
$$

$$
\frac{(m-1)S_2^2}{2\sigma^2}\sim\chi^2(m-1)
$$

$$
F=\frac{\frac{(n-1)S_1^2}{\sigma^2}/(n-1)}{\frac{(m-1)S_2^2}{2\sigma^2}/(m-1)}=\frac{2S_1^2}{S_2^2}\sim F(n-1,m-1)
$$

$$
f'(x)=\left(\frac{x}{3}\sin\frac{x}{3}\right)'=\frac{1}{3}\sin\frac{x}{3}+\frac{x}{3}\cdot\cos\frac{x}{3}\cdot\frac{1}{3}=\frac{1}{3}\sin\frac{x}{3}+\frac{x}{9}\cdot\cos\frac{x}{3}
$$

$$
f'(x)=(-x\sin x)'=-1\cdot\sin x-x\cdot\cos x=-\sin x-x\cdot\cos x
$$

$$
f'_{-}(0)=\lim_{x\to 0^-}\frac{-x\sin x}{x-0}=\lim_{x\to 0^-}-\sin x=0
$$

$$
f'_+(0)=\lim_{x\to0^+}\frac{\frac{x}{3}\sin\frac{x}{3}}{x-0}=\lim_{x\to0^+}\frac{1}{3}\sin\frac{x}{3}=0
$$

$$
f'(0)=f'_{-}(0)=f'_+(0)
$$

$$
\lim_{x\to0^-}f'(x)=\lim_{x\to0^-}-\sin x-x\cos x=0
$$

$$
\lim_{x\to0^+}f'(x)=\lim_{x\to0^+}\frac{1}{3}\sin\frac{x}{3}+\frac{x}{9}\cdot\cos\frac{x}{3}=0
$$

$$ {=0}
f'(0)=\lim_{x\to0^-}f'(x)=\lim_{x\to0^+}f'(x)
$$

$$
\lim_{x\to0^+}f(x)=\lim_{x\to0^+}\frac{x}{3}\sin\frac{x}{3}=0
\\\lim_{x\to0^-}f(x)=\lim_{x\to0^-}-x\sin x=0
\\f(0)=0
\\\lim_{x\to0^+}f(x)=\lim_{x\to0^-}f(x)=f(0)
$$

$$
f''_-(0)=\lim_{x\to0^-}\frac{-\sin x-x\cos x}{x-0}=-2
\\f''_+(0)=\lim_{x\to0^+}\frac{\frac{1}{3}\sin\frac{x}{3}+\frac{x}{9}\cdot\cos\frac{x}{3}}{x-0}=\frac{2}{9}
$$

$$
\gamma=-3 l\left[\begin{array}{l}
1 \\
2 \\
3
\end{array}\right]+l\left[\begin{array}{l}
2 \\
1 \\
1
\end{array}\right]=l\left[\begin{array}{l}
-1 \\
-5 \\
-8
\end{array}\right]=k\left[\begin{array}{l}
1 \\
5 \\
8
\end{array}\right]
$$

$$
A=\left(\begin{array}{ll}
1 &   2  &-2&-1\\
2 &  1  & -5&0\\
3  &  1 &-9 &-1\\
\end{array}\right)\to\left(\begin{array}{ll}
1 &   2  &-2&-1\\
0 &  -3  & -1&2\\
0  &  -5 &-3 &2\\
\end{array}\right)\to\left(\begin{array}{ll}
1 &   2  &-2&-1\\
0 &  3  & 1&-2\\
0  &  5 &3 &-2\\
\end{array}\right)\\
\to\left(\begin{array}{ll}
1 &   8  &0&-5\\
0 &  3  & 1&-2\\
0  &  -4 &0 &4\\
\end{array}\right)\to\left(\begin{array}{ll}
1 &   8  &0&-5\\
0 &  3  & 1&-2\\
0  &  1 &0 &-1\\
\end{array}\right)
\to\left(\begin{array}{ll}
1 &   8  &0&-5\\
0 &  0  & 1&1\\
0  &  1 &0 &-1\\
\end{array}\right)
\to\left(\begin{array}{ll}
1 &   8  &0&-5\\
0  &  1 &0 &-1\\
0 &  0  & 1&1\\
\end{array}\right)
\to\left(\begin{array}{ll}
1 &   0  &0&3\\
0  &  1 &0 &-1\\
0 &  0  & 1&1\\
\end{array}\right)
$$

$$
\alpha=(-3,1,-1,1)^T
$$

$$
\gamma=- l\left[\begin{array}{l}
2 \\
5 \\
9
\end{array}\right]+l\left[\begin{array}{l}
1 \\
0 \\
1
\end{array}\right]=l\left[\begin{array}{l}
-1 \\
-5 \\
-8
\end{array}\right]=k\left[\begin{array}{l}
1 \\
5 \\
8
\end{array}\right]
$$

$$
2^{h-1}-1<n\leq2^h-1\Rightarrow2^{h-1}<n+1\le2^h\Rightarrow h-1<\log_2(n+1)\le h
$$

$$
\left \lfloor x \right \rfloor
$$

$$
\left \lceil x \right \rceil
$$

