# T5

* $$
  f'(x)=2(x-1)(x-3)^2+2(x-1)^2(x-3)\\=(x-1)(x-3)(2x-6+2x-2)\\=4(x-1)(x-2)(x-3)
  $$

* $$
  \Rightarrow f'(1)=f'(2)=f'(3),\\由罗尔定理得，\exist\xi_1\in(1,2),\exist\xi_2\in(2,3)使得f''(\xi_1)=0,f''(\xi_2)=0\\
  $$

* $$
  由于f(x)是四阶表达式，所以f''(x)为二阶表达式\\f''(x)有两个根\xi_1,\xi_2
  $$

* $$
  f''(x)=4(x-2)(x-3)+4(x-1)(x-3)+4(x-1)(x-2)\\=4(3x^2-12x+11)
  $$

* $$
  设f''(x)=12(x-\xi_1)(x-\xi_2),可知在\xi_1,\xi_2左右f''(x)变号
  $$

* $$
  拐点2
  $$

* 



# T4

* $$
  f(x)=ln[2(1+\frac{x}{2})]=ln2+ln(1+\frac{x}{2})\\=ln2+\frac{x}{2}-\frac{1}{2}(\frac{x}{2})^2+\frac{1}{3}(\frac{x}{2})^3+……
  $$

* $$
  ln(1+x)=\sum_{n=1}^{\infty}(-1)^{n-1}\frac{x^n}{n}=x-\frac{1}{2}x^2+\frac{1}{3}x^3-……+(-1)^{n-1}\frac{x^n}{n}+……，-1<x\leq1
  $$

* $$
  lnx^{(n)}=(-1)^{n-1}\frac{(n-1)!}{x^n},x=1,2,……
  $$

* 

